\begin{answer}
We know from the intial assumptions that
\begin{align*}
    p(y^{(i)}=1\mid t^{(i)} = 1, x^{(i)}) = \alpha \\
    p(y^{(i)}=1\mid t^{(i)} = 0, x^{(i)}) = 0
\end{align*}
Using Bayes rule:
\begin{align*}
    &p(t^{(i)}=1\mid y^{(i)} = 1, x^{(i)}) = \frac{p(y^{(i)}=1\mid t^{(i)} = 1, x^{(i)}) \cdot p(t^{(i)}=1, x^{(i)})}{p(y^{(i)}=1, x^{(i)})} \\
    &= \frac{p(y^{(i)}=1\mid t^{(i)} = 1, x^{(i)}) \cdot p(t^{(i)}=1, x^{(i)})}{p(y^{(i)}=1\mid t^{(i)}=1, x^{(i)}) \cdot p(t^{(i)}=1, x^{(i)}) + p(y^{(i)}=1\mid t^{(i)}=0, x^{(i)})\cdot p(t^{(i)}=1, x^{(i)})} \\
    &= \frac{p(y^{(i)}=1\mid t^{(i)} = 1, x^{(i)})}{p(y^{(i)}=1\mid t^{i}=1, x^{(i)}) + p(y^{(i)}=1\mid t^{(i)}=0, x^{(i)})}  \\
    &= \frac{\alpha}{\alpha} = 1 \\
\end{align*}
\end{answer}
