\begin{answer}

Using Bayes theorem:
\begin{equation}
    \label{eq:Bayes}
    p(\theta|x,y) = \frac{p(y|x, \theta)p(\theta)}{p(y)}
\end{equation}
Insert equation~\ref{eq:Bayes} into the definition of the MAP estimator:
\begin{align*}
  \theta_{\text{MAP}} &= \arg\max_\theta p(\theta|x,y) = \arg\max_\theta \frac{p(y|x, \theta)p(\theta)}{p(y)} \\
  &= \arg\max_\theta p(y|x, \theta)p(\theta)
\end{align*}
where the last step utilized that the denominator $p(y)$ does not depend on $\theta$.
\end{answer}
