\begin{answer}
Since the logarithm is a monotonic function, the following equation holds true for $\theta_{\text{MAP}}$:
\begin{align*}
    \theta_{\text{MAP}} = \arg\max_\theta p(y|x, \theta)p(\theta) = -\arg\min_\theta \log\left(p(y|x, \theta)p(\theta)\right)
\end{align*}
Therefore:
\begin{align*}
    \theta_{\text{MAP}} &= - \arg\min_\theta \log\left(p(y|x, \theta)\mathcal{N}(0,\eta^2I)\right) \\
    & = \arg\min_\theta (-\log p(y|x, \theta) - \log(C\cdot e^{\frac{-\theta^T(\eta^2 I)^{-1}\theta}{2}})) \\
    & = \arg\min_\theta (-\log p(y|x, \theta) + \underbrace{\frac{1}{2\eta^2}}_{=\lambda}||\theta||^2_2),
  \end{align*}
  where the normalizatuon constant $C$ could be dropped as it has no effect on the minima with respect to $\theta$.
\end{answer}
