\begin{answer}
Remember the defintion of the conditional probability
\begin{equation*}
    P(Y|X) = \frac{P(X, Y)}{P(X)}
\end{equation*}
Using this, the KL divergence of the joint distributions can be written as:
\begin{align*}
    D_{KL}(P(X,Y)||Q(X,Y)) &= \sum_{x, y} P(x,y)\log{\frac{P(x,y)}{Q(x,y)}}
   = \sum_{x, y} P(x,y)\log{\frac{P(y|x)P(x)}{Q(y|x)Q(x)}} \\
   &= \sum_{x, y} P(x,y)\left(\log{\frac{P(y|x)}{Q(y|x)}} + \log{\frac{P(x)}{Q(x)}} \right) \\
   &= \sum_{x, y} P(x|y)P(y)\log{\frac{P(y|x)}{Q(y|x)}} + \underbrace{\sum_{y} P(y|x)}_{=1} \sum_x P(x) \log{\frac{P(x)}{Q(x)}} \\
   &= D_{KL}(P(Y|X)||Q(Y|X)) + D_{KL}(P(X)||Q(X))
\end{align*}
\hfill \ensuremath{\Box}
\end{answer}
